src/Sound/VCGen/BlockContinuation.dfy
@@ -25,6 +25,25 @@ module Block {
 
     }
 
+    lemma VarsInScopeSuffix(l: nat)
+      requires l <= |this|
+      ensures VarsInScope(l) == this[..l].AllVarsInScope()
+    {
+      if l != 0 {
+        calc {
+          VarsInScope(l);
+        ==
+          this[0].varsInScope + this[1..].VarsInScope(l - 1);
+        == { this[1..].VarsInScopeSuffix(l - 1);
+             assert this[1..][..l - 1] == this[1..l]; }
+          this[0].varsInScope + this[1..l].AllVarsInScope();
+        == { assert this[..l][1..] == this[1..l]; }
+          this[..l].AllVarsInScope();
+        }
+
+      }
+    }
+
     function Size(): nat {
       if this == [] then 0 else SeqSize(this[0].cont) + 1 + this[1..].Size()
     }
@@ -52,41 +71,106 @@ module Block {
         SeqJumpsDefinedOn(this[0].cont, |this[1..]|) && this[1..].JumpsDefined()
     }
 
-    predicate VarsDefined() {
+    predicate VarsDefined(n: nat) 
+      requires IsDefinedOn(n)
+    {
       if this == [] then true else
-        SeqIsDefinedOn(this[0].cont, this[1..].AllVarsInScope()) && this[1..].VarsDefined()
+        SeqIsDefinedOn(this[0].cont, n - this[0].varsInScope) && this[1..].VarsDefined(n - this[0].varsInScope)
     }
 
-    lemma DefinedPrefix'(l: nat)
+    lemma VarsDefinedTransitivity(n1: nat, n2: nat)
+      requires IsDefinedOn(n1)
+      requires VarsDefined(n1)
+      requires n1 <= n2
+      ensures VarsDefined(n2)
+    {
+
+    }
+
+    lemma AllVarsInScopeSuffixSucc(l: nat)
+      requires l < |this|
+      ensures this[..l + 1].AllVarsInScope() == this[..l].AllVarsInScope() + this[l].varsInScope
+      // ensures AllVarsInScope() == this[..l + 1].AllVarsInScope()
+    {
+      VarsInScopeSuffix(l);
+      VarsInScopeLeqAll(l);
+      VarsInScopeLeqAll(l + 1);
+      VarsInScopeSuffix(l + 1);
+    }
+
+    lemma DefinedPrefix''(l: nat, n: nat)
+      requires l <= |this|
+      requires IsDefinedOn(n)
+      ensures n >= this[..l].AllVarsInScope()
+    {
+      VarsInScopeSuffix(l);
+      VarsInScopeLeqAll(l);
+    }
+
+    lemma DefinedPrefix'(l: nat, n: nat)
       requires l < |this|
       requires JumpsDefined()
-      requires VarsDefined()
-      ensures SeqJumpsDefinedOn(this[l].cont, |this[l+1..]|) 
-      ensures SeqIsDefinedOn(this[l].cont, this[l+1..].AllVarsInScope())
+      requires IsDefinedOn(n)
+      requires VarsDefined(n)
+      ensures SeqJumpsDefinedOn(this[l].cont, |this[l + 1..]|) 
+      ensures n >= this[..l + 1].AllVarsInScope()
+      ensures SeqIsDefinedOn(this[l].cont, n - this[..l + 1].AllVarsInScope())
       // ensures SeqIsDefinedOn(this[l].cont, 1000) /*SOUNDNESS BUG:*/
     {
+      DefinedPrefix''(l + 1, n);
       if this != [] {
         if l != 0 {
-          this[1..].DefinedPrefix'(l - 1);
           assert this[1..][l - 1] == this[l];
           assert this[1..][l - 1..] == this[l..];
+          assert this[1..][..l] == this[1..l + 1];
+          this[1..].DefinedPrefix'(l - 1, n - this[0].varsInScope);
+          assert SeqIsDefinedOn(this[l].cont, n - this[0].varsInScope - this[1..l + 1].AllVarsInScope());
+          assert SeqIsDefinedOn(this[l].cont, n - this[..l + 1].AllVarsInScope());
         }
       }
     }
 
-    lemma DefinedPrefix(l: nat)
+    lemma DefinedPrefix(l: nat, n: nat)
       requires l <= |this|
       requires JumpsDefined()
-      requires VarsDefined()
+      requires IsDefinedOn(n)
+      requires VarsDefined(n)
       ensures this[l..].JumpsDefined()
-      ensures this[l..].VarsDefined()
+      ensures n >= this[..l].AllVarsInScope()
+      ensures this[l..].IsDefinedOn(n - this[..l].AllVarsInScope())
+      ensures this[l..].VarsDefined(n - this[..l].AllVarsInScope())
       decreases |this| - l
     {
       if l != 0 {
         if |this| != l {
           assert this[l + 1..] == this[l..][1..];
-          DefinedPrefix(l + 1);
-          DefinedPrefix'(l);
+          assert this[1..][..l - 1] == this[1..l];
+          assert this[1..][..l] == this[1..l + 1];
+          assert this[l..][0] == this[l];
+          DefinedPrefix(l + 1, n);
+          DefinedPrefix'(l, n);
+          assert n >= this[..l+1].AllVarsInScope();
+          assert this[..l+1].AllVarsInScope() == this[..l].AllVarsInScope() + this[l].varsInScope by {
+            AllVarsInScopeSuffixSucc(l);
+          }
+          calc {
+            this[l..].IsDefinedOn(n - this[..l].AllVarsInScope());
+            { VarsInScopeLeqAll(l + 1); }
+            SeqIsDefinedOn(this[l].cont, n - this[..l].AllVarsInScope()) && 
+              this[l+1..].IsDefinedOn(n - this[..l].AllVarsInScope() - this[l].varsInScope);
+            true;
+          }
+          var m := n - this[..l].AllVarsInScope();
+          calc {
+            this[l..].VarsDefined(m);
+            SeqIsDefinedOn(this[l].cont, n - this[..l + 1].AllVarsInScope()) && 
+            this[l + 1..].VarsDefined(n - this[..l + 1].AllVarsInScope());
+            SeqIsDefinedOn(this[l].cont, n - this[..l + 1].AllVarsInScope());
+            true;
+          }
+        } else {
+          VarsInScopeLeqAll(|this|);
+          VarsInScopeSuffix(|this|);
         }
       }
     }
